Deque.v
@@ -1,0 +1,660 @@
+Add Rec LoadPath "/home/zeimer/Code/Coq".
+
+Require Import RCCBase.
+
+Definition Deque (A : Type) : Type := list A * list A.
+
+(* Auxiliary function that restores balance. *)
+Require Import Div2.
+
+Function split {A : Type} (n : nat) (l : list A) : list A * list A :=
+match n, l with
+    | 0, _ => ([], l)
+    | _, [] => ([], [])
+    | S n', h :: t =>
+        let '(f, r) := split n' t in (h :: f, r)
+end.
+
+Definition halve {A : Type} (l : list A) : list A * list A :=
+  split (div2 (length l)) l.
+
+Function deque {A : Type} (f r : list A) : Deque A :=
+match f, r with
+    | [], [] => (f, r)
+    | [], [_] => (f, r)
+    | [], _ => let '(r, f) := halve r in (rev f, r)
+    | [_], [] => (f, r)
+    | _, [] => let '(f, r) := halve f in (f, rev r)
+    | _, _ => (f, r)
+end.
+
+Definition empty {A : Type} : Deque A := ([], []).
+
+Function isEmpty {A : Type} (d : Deque A) : bool :=
+match d with
+    | ([], []) => true
+    | _ => false
+end.
+
+Definition cons {A : Type} (x : A) (d : Deque A) : Deque A :=
+  let '(f, r) := d in deque (x :: f) r.
+
+Function head {A : Type} (d : Deque A) : option A :=
+match d with
+    | ([], []) => None
+    | ([], [h]) => Some h
+    | ([], _) => None
+    | (h :: _, _) => Some h
+end.
+
+Function tail {A : Type} (d : Deque A) : option (Deque A) :=
+match d with
+    | ([], []) => None
+    | ([], [_]) => Some empty
+    | ([], _) => None
+    | (_ :: t, r) => Some (deque t r)
+end.
+
+Definition snoc {A : Type} (x : A) (d : Deque A) : Deque A :=
+  let '(f, r) := d in deque f (x :: r).
+
+Function last {A : Type} (d : Deque A) : option A :=
+match d with
+    | ([], []) => None
+    | ([x], []) => Some x
+    | (_, []) => None
+    | (_, x :: _) => Some x
+end.
+
+Function init {A : Type} (d : Deque A) : option (Deque A) :=
+match d with
+    | ([], []) => None
+    | ([_], []) => Some empty
+    | (_, []) => None
+    | (f, _ :: t) => Some (deque f t)
+end.
+
+(** Lemmas for [deque]. *)
+Lemma split_inv_l :
+  forall (A : Type) (n : nat) (l r : list A),
+    split n l = ([], r) -> n = 0 \/ (l = [] /\ r = []).
+Proof.
+  intros. functional induction @split A n l.
+    left. reflexivity.
+    right. inv H.
+    inv H.
+Qed.
+
+Lemma split_inv_r :
+  forall (A : Type) (n : nat) (l f : list A),
+    split n l = (f, []) -> length l <= n \/ l = [] /\ f = [].
+Proof.
+  intros. functional induction @split A n l; cbn; inv H.
+    left. apply le_n_S. destruct (IHp _ e1).
+      assumption.
+      inv H. cbn. apply le_0_n.
+Qed.
+
+Functional Scheme div2_ind := Induction for div2 Sort Prop.
+
+Lemma div2_inv_aux :
+  forall n : nat, n <> 0 -> ~ n <= div2 n.
+Proof.
+  intros. functional induction div2 n.
+    contradiction.
+    intro. inv H0.
+    intro. apply le_S_n in H0. destruct n'.
+      cbn in H0. inv H0.
+      assert (S n' <> 0) by congruence. specialize (IHn0 H1).
+        assert (S n' <= Init.Nat.div2 (S n')) by omega. contradiction.
+Qed.
+
+Lemma div2_inv :
+  forall n : nat, n <= div2 n -> n = 0.
+Proof.
+  intros. destruct n.
+    trivial.
+    assert (H' := div2_inv_aux (S n) ltac:(inversion 1)).
+      contradiction.
+Qed.
+
+(* The Deque invariant and proofs that the operation maintain it. *)
+Definition isDeque {A : Type} (d : Deque A) : Prop :=
+  let '(f, r) := d in 2 <= length f + length r -> f <> [] /\ r <> [].
+
+Lemma empty_isDeque :
+  forall A : Type, isDeque (@empty A).
+Proof.
+  cbn. inversion 1.
+Qed.
+
+Lemma deque_isDeque :
+  forall (A : Type) (f r : list A), isDeque (deque f r).
+Proof.
+  intros. functional induction @deque A f r; cbn; intros; try omega.
+    destruct f0.
+      destruct (split_inv_r _ _ _ _ e1).
+        apply div2_inv in H0. destruct r; inv H0.
+        destruct H0; subst; cbn in *. contradiction.
+      destruct r0.
+        apply split_inv_l in e1. destruct e1.
+          destruct r as [| h1 [| h2 t]]; cbn in *; firstorder.
+          inv H0.
+        case_eq (rev (a :: f0)); intros.
+          cbn in H0. apply app_eq_nil in H0. inv H0. inv H2.
+          split; congruence.
+    destruct f0.
+      destruct (split_inv_l _ _ _ _ e1).
+        destruct f as [| h1 [| h2 t]]; cbn in *; firstorder.
+        inv H0.
+      destruct r0.
+        apply split_inv_r in e1. destruct e1.
+          apply div2_inv in H0.
+            destruct f as [| h1 [| h2 t]]; cbn in *; firstorder.
+          inv H0.
+        case_eq (rev (a0 :: r0)); intros.
+          cbn in H0. apply app_eq_nil in H0. inv H0. inv H2.
+          split; congruence.
+    destruct f as [| hf1 [| hf2 tf]], r as [| hr1 [| hr2 tr]]; cbn in *;
+      firstorder.
+Qed.
+
+(*Restart.
+  intros. functional induction @deque A f r; cbn; intros;
+  try omega; unfold halve in *.
+    functional inversion e1;
+    repeat match goal with
+        | H : existT _ _ _ = _ |- _ => apply inj_pair2 in H
+    end; subst.
+      destruct f0 as [| h1 [| h2 t]]; cbn in *; firstorder.
+      inv H.
+      destruct t.
+        contradiction.
+        cbn in *.*)
+
+Lemma cons_isDeque :
+  forall (A : Type) (x : A) (d : Deque A), isDeque (cons x d).
+Proof.
+  destruct d. apply deque_isDeque.
+Qed.
+
+Lemma tail_isDeque :
+  forall (A : Type) (x : A) (d d' : Deque A),
+    tail d = Some d' -> isDeque d'.
+Proof.
+  intros. functional induction @tail A d; inv H.
+    apply empty_isDeque.
+    apply deque_isDeque.
+Qed.
+
+Lemma snoc_isDeque :
+  forall (A : Type) (x : A) (d : Deque A), isDeque (snoc x d).
+Proof.
+  destruct d. apply deque_isDeque.
+Qed.
+
+Lemma init_isDeque :
+  forall (A : Type) (x : A) (d d' : Deque A),
+    init d = Some d' -> isDeque d'.
+Proof.
+  intros. functional induction @init A d; inv H.
+    apply empty_isDeque.
+    apply deque_isDeque.
+Qed.
+
+(* Properties of [isEmpty]. *)
+Lemma isEmpty_deque :
+  forall (A : Type) (f r : list A),
+    isEmpty (deque f r) = true -> f = [] /\ r = [].
+Proof.
+  intros. functional induction @deque A f r;
+  cbn in *; auto; try congruence.
+    destruct f0.
+      destruct (split_inv_r _ _ _ _ e1).
+        apply div2_inv in H0. destruct r; inv H0.
+        tauto.
+      case_eq (rev (a :: f0)); intros.
+        cbn in H0. apply app_eq_nil in H0. destruct H0. congruence.
+        rewrite H0 in H. congruence.
+    destruct f0.
+      destruct (split_inv_l _ _ _ _ e1).
+        destruct f as [| h1 [| h2 t]]; cbn in *; firstorder.
+        inv H0.
+      congruence.
+    destruct f as [| h1 [| h2 t]], r; firstorder.
+Qed.
+
+Lemma isEmpty_cons :
+  forall (A : Type) (x : A) (d : Deque A),
+    isEmpty (cons x d) = false.
+Proof.
+  destruct d as [f r]. unfold cons.
+  case_eq (isEmpty (deque (x :: f) r)); intros.
+    apply isEmpty_deque in H. inv H. congruence.
+    reflexivity.
+Qed.
+
+Lemma isEmpty_head_false :
+  forall (A : Type) (h : A) (d : Deque A),
+    head d = Some h -> isEmpty d = false.
+Proof.
+  intros. functional induction @head A d; inv H.
+Qed.
+
+Lemma isEmpty_head_true :
+  forall (A : Type) (d : Deque A),
+    isEmpty d = true -> head d = None.
+Proof.
+  intros. functional inversion H. reflexivity.
+Qed.
+
+Lemma isEmpty_tail_false :
+  forall (A : Type) (d : Deque A),
+    isEmpty d = true -> tail d = None.
+Proof.
+  intros. destruct d. functional inversion H; subst. reflexivity.
+Qed.
+
+Lemma isEmpty_tail_true :
+  forall (A : Type) (d d' : Deque A),
+    tail d = Some d' -> isEmpty d = false.
+Proof.
+  intros. destruct d. functional inversion H; subst; reflexivity.
+Qed.
+
+Lemma isEmpty_snoc :
+  forall (A : Type) (x : A) (d : Deque A),
+    isEmpty (snoc x d) = false.
+Proof.
+  destruct d as [f r]. unfold snoc.
+  case_eq (isEmpty (deque f (x :: r))); intros.
+    apply isEmpty_deque in H. inv H. congruence.
+    reflexivity.
+Qed.
+
+Lemma isEmpty_last_false :
+  forall (A : Type) (h : A) (d : Deque A),
+    last d = Some h -> isEmpty d = false.
+Proof.
+  intros. functional induction @last A d; inv H.
+  destruct _x; reflexivity.
+Qed.
+
+Lemma isEmpty_last_true :
+  forall (A : Type) (d : Deque A),
+    isEmpty d = true -> last d = None.
+Proof.
+  intros. functional inversion H. reflexivity.
+Qed.
+
+Lemma isEmpty_init_false :
+  forall (A : Type) (d : Deque A),
+    isEmpty d = true -> init d = None.
+Proof.
+  intros. destruct d. functional inversion H; subst. reflexivity.
+Qed.
+
+Lemma isEmpty_init_true :
+  forall (A : Type) (d d' : Deque A),
+    init d = Some d' -> isEmpty d = false.
+Proof.
+  intros. destruct d. functional inversion H; subst; cbn.
+    reflexivity.
+    destruct l; reflexivity.
+Qed.
+
+(* [size] and it's properties *)
+Definition size {A : Type} (d : Deque A) : nat :=
+  let '(f, r) := d in length f + length r.
+
+Lemma size_empty :
+  forall A : Type, size (@empty A) = 0.
+Proof. reflexivity. Qed.
+
+Lemma size_deque :
+  forall (A : Type) (f r : list A),
+    size (deque f r) = length f + length r.
+Proof.
+  intros. functional induction @deque A f r; cbn; try congruence.
+    unfold halve in e1. clear y.
+      functional induction @split A (Nat.div2 (length r)) r; inv e1; cbn.
+        rewrite rev_length, <- plus_n_O. reflexivity.
+        specialize (IHp _ _ e2). omega.
+    unfold halve in e1. clear y.
+      functional induction @split A (Nat.div2 (length f)) f; inv e1; cbn.
+        rewrite <- plus_n_O. apply rev_length.
+        specialize (IHp _ _ e2). omega.
+Qed.
+
+Lemma size_cons :
+  forall (A : Type) (x : A) (d : Deque A),
+    size (cons x d) = S (size d).
+Proof.
+  intros. unfold cons. destruct d. rewrite size_deque. cbn. reflexivity.
+Qed.
+
+Lemma size_tail :
+  forall (A : Type) (d d' : Deque A),
+    tail d = Some d' -> size d' = pred (size d).
+Proof.
+  intros. functional inversion H; subst.
+    reflexivity.
+    rewrite size_deque. cbn. reflexivity.
+Qed.
+
+Lemma size_snoc :
+  forall (A : Type) (x : A) (d : Deque A),
+    size (snoc x d) = S (size d).
+Proof.
+  intros. unfold snoc. destruct d. rewrite size_deque. cbn. omega.
+Qed.
+
+Lemma size_init :
+  forall (A : Type) (d d' : Deque A),
+    init d = Some d' -> size d' = pred (size d).
+Proof.
+  intros. functional inversion H; subst.
+    reflexivity.
+    rewrite size_deque. cbn. omega.
+Qed.
+
+(* [map] and its properties *)
+Definition fmap {A B : Type} (f : A -> B) (d : Deque A) : Deque B :=
+  let '(front, rear) := d in (map f front, map f rear).
+
+Lemma fmap_empty :
+  forall (A B : Type) (f : A -> B),
+    fmap f (@empty A) = @empty B.
+Proof. reflexivity. Qed.
+
+Lemma fmap_isEmpty :
+  forall (A B : Type) (f : A -> B) (d : Deque A),
+    isEmpty (fmap f d) = isEmpty d.
+Proof.
+  intros. functional induction @isEmpty A d; cbn.
+    reflexivity.
+    destruct d, l, l0; cbn; firstorder.
+Qed.
+
+Lemma map_split :
+  forall (A B : Type) (f : A -> B) (n : nat) (l l1 l2 : list A),
+    split n l = (l1, l2) -> split n (map f l) = (map f l1, map f l2).
+Proof.
+  intros. functional induction @split A n l; cbn; inv H.
+    destruct n; reflexivity.
+    rewrite (IHp _ _ _ e1). cbn. reflexivity.
+Qed.
+
+Lemma map_split' :
+  forall (A B : Type) (f : A -> B) (n : nat) (l : list A),
+    split n (map f l) = (map f (fst (split n l)), map f (snd (split n l))).
+Proof.
+  intros. case_eq (split n l); cbn; intros.
+  apply map_split. assumption.
+Qed.
+
+Lemma fmap_deque :
+  forall (A B : Type) (g : A -> B) (f r : list A),
+    fmap g (deque f r) = deque (map g f) (map g r).
+Proof.
+  intros. functional induction @deque A f r; cbn;
+  auto; unfold halve in *.
+    rewrite ?map_length, map_split'. destruct r as [| h1 [| h2 t]]; cbn.
+      contradiction.
+      contradiction.
+      cbn in *. destruct (split (Nat.div2 (length t)) (h2 :: t)).
+        inv e1. cbn. rewrite map_rev. reflexivity.
+    destruct f as [| h1 [| h2 t]].
+      contradiction.
+      contradiction.
+      cbn in *. change (g h2 :: map g t) with (map g (h2 :: t)).
+        rewrite ?map_length, map_split'.
+        destruct (split (Nat.div2 (length t)) (h2 :: t)).
+        inv e1. cbn. rewrite map_rev. reflexivity.
+    destruct f as [| hf1 [| hf2 tf]], r as [| hr1 [| hr2 tr]]; cbn;
+    firstorder.
+Qed.
+
+Lemma fmap_cons :
+  forall (A B : Type) (f : A -> B) (x : A) (d : Deque A),
+    fmap f (cons x d) = cons (f x) (fmap f d).
+Proof.
+  unfold cons at 1. destruct d. rewrite fmap_deque. reflexivity.
+Qed.
+
+Lemma fmap_head :
+  forall (A B : Type) (f : A -> B) (d : Deque A),
+    head (fmap f d) =
+    match head d with
+        | None => None
+        | Some x => Some (f x)
+    end.
+Proof.
+  intros. functional induction @head A d; cbn; try reflexivity.
+  destruct _x as [| h1 [| h2 t]]; cbn; tauto.
+Qed.
+
+Lemma fmap_tail :
+  forall (A B : Type) (f : A -> B) (d d' : Deque A),
+    tail d = Some d' -> tail (fmap f d) = Some (fmap f d').
+Proof.
+  intros. functional induction @tail A d; cbn; inv H.
+  f_equal. rewrite fmap_deque. reflexivity.
+Qed.
+
+Lemma fmap_snoc :
+  forall (A B : Type) (f : A -> B) (x : A) (d : Deque A),
+    fmap f (snoc x d) = snoc (f x) (fmap f d).
+Proof.
+  unfold snoc at 1. destruct d. rewrite fmap_deque. reflexivity.
+Qed.
+
+Lemma fmap_last :
+  forall (A B : Type) (f : A -> B) (d : Deque A),
+    last (fmap f d) =
+    match last d with
+        | None => None
+        | Some x => Some (f x)
+    end.
+Proof.
+  intros. functional induction @last A d; cbn; try reflexivity.
+  all: destruct _x as [| h1 [| h2 t]]; cbn; tauto.
+Qed.
+
+Lemma fmap_init :
+  forall (A B : Type) (f : A -> B) (d d' : Deque A),
+    init d = Some d' -> init (fmap f d) = Some (fmap f d').
+Proof.
+  intros. functional induction @init A d; cbn; inv H.
+  case_eq (map f f0); intros.
+    f_equal. assert (f0 = []) by (destruct f0; inv H). subst.
+      rewrite fmap_deque. reflexivity.
+    rewrite fmap_deque, H. destruct l; reflexivity.
+Qed.
+
+Lemma fmap_size :
+  forall (A B : Type) (f : A -> B) (d : Deque A),
+    size (fmap f d) = size d.
+Proof.
+  destruct d. cbn. rewrite ?map_length. reflexivity.
+Qed.
+
+(* Properties of [head]. *)
+(*Lemma head_deque :
+  forall (A : Type) (f r : list A),
+    head (deque f r) =
+    match f, r with
+        | 
+Proof.
+  intros. functional induction @deque A f r; cbn; auto;
+  unfold halve in *.
+    functional induction @split A (Nat.div2 (length r)) r; inv e1.
+      destruct f0 as [| h1 [| h2 t]]; cbn; firstorder.
+  
+    match f, r with
+        | [], [] => None
+        | [], *)
+
+Lemma head_empty :
+  forall A : Type, head (@empty A) = None.
+Proof. reflexivity. Qed.
+
+Lemma head_cons :
+  forall (A : Type) (x : A) (d : Deque A),
+    head (cons x d) = Some x.
+Proof.
+  destruct d as [f r]. unfold cons.
+  functional induction @deque A (x :: f) r; cbn.
+Abort.
+
+(* [toList] and its properties. *)
+Definition toList {A : Type} (d : Deque A) : list A :=
+  let '(f, r) := d in f ++ rev r.
+
+Lemma toList_deque :
+  forall (A : Type) (f r : list A),
+    toList (deque f r) = f ++ rev r.
+Proof.
+  intros. functional induction @deque A f r; cbn; auto;
+  unfold halve in *.
+    clear y. functional induction @split A (Nat.div2 (length r)) r; inv e1; cbn.
+      apply app_nil_r.
+      rewrite app_assoc, (IHp _ _ e2). reflexivity.
+    clear y. functional induction @split A (Nat.div2 (length f)) f; inv e1; cbn.
+      rewrite rev_involutive, app_nil_r. reflexivity.
+      rewrite (IHp _ _ e2). reflexivity.
+Qed.
+
+Lemma toList_empty :
+  forall A : Type, toList (@empty A) = [].
+Proof. reflexivity. Qed.
+
+Lemma toList_cons :
+  forall (A : Type) (x : A) (d : Deque A),
+    toList (cons x d) = x :: toList d.
+Proof.
+  destruct d. unfold cons. rewrite toList_deque. cbn. reflexivity.
+Qed.
+
+Lemma toList_head :
+  forall (A : Type) (d : Deque A),
+    isDeque d ->
+    head d =
+    match toList d with
+        | [] => None
+        | h :: _ => Some h
+    end.
+Proof.
+  intros. functional induction @head A d; cbn; auto.
+  cbn in H. destruct _x as [| h1 [| h2 t]]; cbn; try tauto.
+  cbn in *. destruct H.
+    omega.
+    contradiction.
+Qed.
+
+Lemma toList_tail :
+  forall (A : Type) (d d' : Deque A),
+    tail d = Some d' -> toList d' =
+    match toList d with
+        | [] => toList d'
+        | _ :: t => t
+    end.
+Proof.
+  intros. functional induction @tail A d; cbn; inv H.
+  rewrite toList_deque. reflexivity.
+Qed.
+
+Lemma toList_snoc :
+  forall (A : Type) (x : A) (d : Deque A),
+    toList (snoc x d) = toList d ++ [x].
+Proof.
+  destruct d. unfold cons. cbn. rewrite toList_deque. cbn.
+  rewrite app_assoc. reflexivity.
+Qed.
+
+Lemma toList_last :
+  forall (A : Type) (d : Deque A), isDeque d ->
+    last d =
+    match rev (toList d) with
+        | [] => None
+        | h :: _ => Some h
+    end.
+Proof.
+  intros. functional induction @last A d; cbn; auto.
+    cbn in H. destruct _x as [| h1 [| h2 t]]; cbn; try tauto.
+      cbn in *. destruct H. omega. contradiction.
+    case_eq (rev (_x ++ rev _x0 ++ [x])); intros;
+      rewrite !rev_app_distr in H0; cbn in *; congruence.
+Qed.
+
+Lemma toList_init :
+  forall (A : Type) (d d' : Deque A),
+    init d = Some d' -> toList d' =
+    match rev (toList d) with
+        | [] => []
+        | _ :: t => rev t
+    end.
+Proof.
+  intros. functional induction @init A d; cbn; inv H.
+  rewrite toList_deque. rewrite !rev_app_distr. cbn.
+  rewrite rev_app_distr, !rev_involutive. reflexivity.
+Qed.
+
+Lemma toList_size :
+  forall (A : Type) (d : Deque A),
+    size d = length (toList d).
+Proof.
+  destruct d as [f r]. unfold size. cbn.
+  rewrite app_length, rev_length. reflexivity.
+Qed.
+
+(* [drev] (deque reversion) and its properties. *)
+Definition drev {A : Type} (d : Deque A) : Deque A :=
+  let '(f, r) := d in (r, f).
+
+Lemma drev_spec :
+  forall (A : Type) (d : Deque A),
+    toList (drev d) = rev (toList d).
+Proof.
+  destruct d. cbn. rewrite rev_app_distr, rev_involutive. reflexivity.
+Qed.
+
+Lemma drev_inv :
+  forall (A : Type) (d : Deque A), drev (drev d) = d.
+Proof. destruct d; reflexivity. Qed.
+
+Compute drev (deque [1] [2; 3]).
+Compute deque [1; 2] [].
+
+Lemma drev_deque :
+  forall (A : Type) (f r : list A),
+    drev (deque f r) = deque r f.
+Proof.
+  intros. functional induction @deque A f r; cbn; auto;
+  unfold halve in *.
+    Focus 3.
+      destruct f as [| hf1 [| hf2 t]], r as [| hr1 [| hr2 tr]]; cbn; firstorder.
+    Focus 2.
+    functional induction @split A (Nat.div2 (length f)) f; inv e1.
+      destruct r0 as [| h1 [| h2 t]]; cbn; try contradiction.
+        rewrite <- app_assoc. reflexivity.
+      destruct t; firstorder.
+    functional induction @split A (Nat.div2 (length r)) r; inv e1.
+      destruct f0 as [| h1 [| h2 t]]; cbn; try contradiction.
+        case_eq (split (Nat.div2 (length t)) (h2 :: t)); intros.
+Admitted.
+
+Lemma drev_cons :
+  forall (A : Type) (x : A) (d : Deque A),
+    drev (cons x d) = snoc x (drev d).
+Proof.
+  destruct d as [f r]. unfold cons. rewrite drev_deque. cbn. reflexivity.
+Qed.
+
+Lemma drev_head :
+  forall (A : Type) (d : Deque A),
+    head (drev d) = last d.
+Proof.
+  intros. functional induction @head A d; cbn; auto.
+  destruct _x0, _x; reflexivity.
+Qed.
